prove jump_recIn

Computability/Jump.lean
@@ -45,7 +45,8 @@ Its domain is the set of n where the n-th oracle program halts on input n with o
 problem relative to f.
 -/
 def jump (f : ℕ →. ℕ) : ℕ →. ℕ :=
-  λ n => evalo (λ _ : Unit => f) (decodeCodeo n) n
+  -- λ n => evalo (λ _ : Unit => f) (decodeCodeo n) n
+  λ n => evalo (λ _ : Unit => f) (decodeCodeo (Nat.unpair n).1) (Nat.unpair n).2
 
 /-
 The oracle corresponding to a decidable set A ⊆ ℕ, returning 0 on elements of A and undefined elsewhere.
@@ -75,7 +76,67 @@ abbrev W [Primcodable α] (e : ℕ) (f : α → ℕ →. ℕ) := (evalo f (decod
 
 notation:100 f"⌜" => jump f
 
-theorem jump_recIn (f : ℕ →. ℕ) : f ≤ᵀ (f⌜) := by sorry
+variable {α : Type*} {β : Type*} {σ : Type*}
+variable [Primcodable α] [Primcodable β] [Primcodable σ]
+theorem Primrec.projection {f : α → β → σ} {a:α} (h:Primrec₂ f) : Primrec (f a) := by
+  refine Primrec₂.comp h ?_ ?_
+  · exact const a
+  · exact Primrec.id
+
+
+
+
+
+
+-- theorem jump_recIn (f : ℕ →. ℕ) : f ≤ᵀ (f⌜) := by sorry
+theorem jump_recIn (f : ℕ →. ℕ) : f ≤ᵀ (f⌜) := by
+  have main: RecursiveIn {jump f} (f) := by
+    have giseq: f = (fun x => Nat.pair (encodeCodeo (codeo.oracle 0)) x >>= (jump f)) := by
+      funext xs
+      simp
+      rw [jump]
+      simp
+      rw [decodeCodeo.eq_def]
+      simp
+      constructor
+
+    nth_rewrite 2 [giseq]
+    apply RecursiveIn.comp
+    · constructor
+      simp
+    · simp
+      apply Nat.Partrec.recursiveIn
+      refine Partrec.nat_iff.mp ?_
+      refine Partrec.comp ?_ ?_
+      · exact Partrec.some
+      · refine Primrec.to_comp ?_
+        rw [encodeCodeo]
+        simp
+        exact Primrec.projection Primrec₂.natPair
+
+
+
+    -- sorry
+  exact main
+
+theorem k0lek (f : ℕ →. ℕ) : (f⌜) ≤ᵀ  (λ n => evalo (λ _ : Unit => f) (decodeCodeo n) n) := by
+  let k := λ n => evalo (λ _ : Unit => f) (decodeCodeo n) n
+  let h := λ (ex:ℕ) => encodeCodeo (codeo.comp (decodeCodeo ex.unpair.1) (const ex.unpair.2))
+  -- h takes as input (e,x), and outputs the index for the function which calculates and returns [e:f](x).
+  -- which is... encodeCodeo (codeo.comp (decodeCodeo e) (codeo.succ codeo.succ ... codeo.zero))
+  -- which is... encodeCodeo (codeo.comp (decodeCodeo e) (const x))
+  have k0_intermsof_k : f⌜ = k ∘ h := by
+    simp [k, h]
+    rw [@Function.comp_def]
+    simp [decodeCodeo_encodeCodeo]
+    simp [evalo]
+    simp [evalo_const]
+    exact rfl
+  simp [k0_intermsof_k]
+  sorry
+
+
+
 
 theorem jump_not_reducible (f : ℕ →. ℕ) : ¬(f⌜ ≤ᵀ f) := by sorry
 
