Computability/hy.lean
@@ -1,0 +1,8 @@
+-- some theorems that'd be nice:
+-- 1. K_0 =_T K
+-- 2. characterising the c.e. sets as domains of partial functions is equivalent to characterising them as ranges of partial functions
+-- 3. Non-empty c.e. sets are totally generatable
+-- 4. the non constructive thm: Theorem 5.11: see /mnt/Q/Mathematics/LaTeX/Textbooks/ToRFaEC.pdf
+-- there exists an infinite set having no infinite recursively enumerable subset. (problem 5.8 ToRFaEC)
+
+-- THEOREM 10.3.5 of /mnt/Q/Mathematics/Textbooks/Computability/Computability Theory [Cooper] (2004).pdf
